Towards kinder notations for well-typed processes

theories/AtomSets.v
@@ -15,8 +15,10 @@ Notation atom:=avar.t.
 
 Notation rvar := (lnvar atom).
 
-Module Lbl := NewAtom def_atom.
-Notation lbl := Lbl.t.
+(* Module Lbl := NewAtom def_atom. *)
+(* Notation lbl := Lbl.t. *)
+Definition lbl := nat.
+(* Notation mk_lbl := Lbl.mk_atom. *)
 
 (* Supported messages *)
 Inductive mty : Type :=
@@ -41,18 +43,14 @@ Fixpoint mty_eq (m1 m2 : mty) : bool :=
 
 Lemma mty_eqP t1 t2 : reflect (t1 = t2) (mty_eq t1 t2).
 Proof.
-(*   elim: t1 t2 => [|||l1 Ihl r1 Ihr|l1 Ihl r1 Ihr|t1 Ih] *)
-(*                    [|||l2 r2|l2 r2| t2]/=; try by constructor. *)
-(*   - case: Ihl=>[<-|E]/=; last by constructor=>[[/E]]. *)
-(*     case: Ihr=>[<-|E]/=; last by constructor=>[[/E]]. *)
-(*     by constructor. *)
-(*   - case: Ihl=>[<-|E]/=; last by constructor=>[[/E]]. *)
-(*     case: Ihr=>[<-|E]/=; last by constructor=>[[/E]]. *)
-(*     by constructor. *)
-(*   - case: Ih =>[<-|E]/=; last by constructor=>[[/E]]. *)
-(*     by constructor. *)
-(* Qed. *)
-Admitted.
+  elim: t1 t2=>[|||l1 Ihl r1 Ihr|l1 Ihl r1 Ihr] [|||l2 r2|l2 r2]/=; try by constructor.
+  - case: Ihl=>[<-|E]/=; last by constructor=>[][].
+    case: Ihr=>[<-|E]/=; last by constructor=>[][].
+    by constructor.
+  - case: Ihl=>[<-|E]/=; last by constructor=>[][].
+    case: Ihr=>[<-|E]/=; last by constructor=>[][].
+    by constructor.
+Qed.
 
 Definition mty_eqMixin := EqMixin mty_eqP.
 Canonical mty_eqType := Eval hnf in EqType mty mty_eqMixin.
@@ -67,67 +65,48 @@ Fixpoint coq_ty m :=
   (* | T_seq l => seq (coq_ty l) *)
   end%type.
 
-Definition eq_coq_ty {T} (m : coq_ty T) (n : coq_ty T) : bool.
-  move: m n.
-  elim: T ; try( move=>m n ;refine (m==n)).
+Fixpoint eq_coq_ty' {T} : coq_ty T -> coq_ty T -> bool
+  := match T with
+     | T_nat => fun n m => n == m
+     | T_bool => fun n m => n == m
+     | T_unit => fun n m => n == m
+     | T_sum Tl Tr =>
+       fun n m =>
+         match n, m with
+         | inl x, inl y => eq_coq_ty' x y
+         | inr x, inr y => eq_coq_ty' x y
+         | _, _ => false
+         end
+     | T_prod Tl Tr =>
+       fun n m =>
+         match n, m with
+         | (x1, x2), (y1, y2) => eq_coq_ty' x1 y1 && eq_coq_ty' x2 y2
+         end
+     end.
 
-  {
-    move=> Tl Eql Tr Eqr m n.
-
-    elim m ; elim n.
-
-    apply Eql.
-
-    move=> _ _. apply false.
-    move=> _ _. apply false.
-
-    apply Eqr.
-  }
-
-  {
-    move=> Tl Eql Tr Eqr m n.
-
-    case m=>ml mr.
-    case n=>nl nr.
-    refine (_ && _).
-
-    apply: Eql.
-    apply: ml.
-    apply: nl.
-
-    apply: Eqr.
-    apply: mr.
-    apply: nr.
-  }
-
-Defined.
-
-  (* := *)
-  (* match T with *)
-  (* | T_nat => fun m n => m == n *)
-  (* (* | T_bool => fun m n => m == n *) *)
-  (* (* | T_unit => fun m n => m == n *) *)
-  (* (* | T_sum l r => _ *) *)
-  (* (* | T_prod l r => _ *) *)
-  (* (* | T_seq l => _ *) *)
-
-  (* end m n. *)
-
-
-Lemma coq_ty_eqP {T} : Equality.axiom (@eq_coq_ty T).
+Lemma coq_ty_eqP' {T} : Equality.axiom (@eq_coq_ty' T).
 Proof.
-  move=>x. move: x.
-  elim T=>//= ; try (intros ; apply eqP).
-  (* these two cases turn horrendous because of the tactic based function definition *)
-Admitted.
+  elim: T=>[|||Tl Ihl Tr Ihr|Tl Ihl Tr Ihr]/=x y; try by apply/eqP.
+  - case: x=>x; case: y=>y/=; try by constructor.
+    + by case: Ihl=>[<-|E]; constructor=>//[][].
+    + by case: Ihr=>[<-|E]; constructor=>//[][].
+  - case: x=>[x1 x2]; case: y=>[y1 y2]/=.
+    case: Ihl=>[<-|E]/=; try by constructor=>[][].
+    case: Ihr=>[<-|E]/=; try by constructor=>[][].
+    by constructor.
+Qed.
 
-Definition coq_ty_eqMixin {T} := EqMixin (@coq_ty_eqP T).
+Definition coq_ty_eqMixin {T} := EqMixin (@coq_ty_eqP' T).
 Canonical coq_ty_eqType {T} := Eval hnf in EqType (coq_ty T) coq_ty_eqMixin.
 
-Definition g_prefix := ((role * role) * mty)%type.
+Definition eq_coq_ty {T1 T2} : coq_ty T1 -> coq_ty T2 -> bool :=
+  match @eqP _ T1 T2 with
+  | ReflectT H =>
+    match H with
+    | erefl => eq_coq_ty'
+    end
+  | ReflectF _ =>
+    fun _ _ => false
+  end.
 
-(*
- Parameter mty_lbl : mty -> seq lbl.
- Parameter lbl_mty : seq lbl -> mty.
- Parameter lbl_mty_iso : forall l t, (lbl_mty l == t) = (l == mty_lbl t).
-*)
+Definition g_prefix := ((role * role) * mty)%type.
